pcuic/theories/PCUICClosed.v
@@ -1,5 +1,5 @@
 (* Distributed under the terms of the MIT license.   *)
-
+From Equations Require Import Equations.
 From Coq Require Import Bool String List Program BinPos Compare_dec Arith Lia.
 From Template Require Import config utils Ast.
 From PCUIC Require Import PCUICAst PCUICAstUtils PCUICInduction PCUICLiftSubst PCUICUnivSubst PCUICTyping PCUICWeakeningEnv.
@@ -8,8 +8,10 @@ Require Import ssreflect ssrbool.
 Definition closed_decl n d :=
   option_default (closedn n) d.(decl_body) true && closedn n d.(decl_type).
 
-Definition closed_ctx ctx :=
-  forallb id (mapi (fun k d => closed_decl k d) (List.rev ctx)).
+Definition closedn_ctx n ctx :=
+  forallb id (mapi (fun k d => closed_decl (n + k) d) (List.rev ctx)).
+
+Notation closed_ctx ctx := (closedn_ctx 0 ctx).
 
 (** * Lemmas about the [closedn] predicate *)
 
@@ -144,7 +146,86 @@ Proof.
     do 3 (f_equal; intuition eauto).
 Qed.
 
-Require Import ssreflect.
+Arguments skipn : simpl never.
+
+Lemma destArity_spec ctx T :
+  match destArity ctx T with
+  | Some (ctx', s) => it_mkProd_or_LetIn ctx T = it_mkProd_or_LetIn ctx' (tSort s)
+  | None => True
+  end.
+Proof.
+  induction T in ctx |- *; simpl; simplify_dep_elim; try easy.
+  specialize (IHT2 (ctx,, vass n T1)). now destruct destArity.
+  specialize (IHT3 (ctx,, vdef n T1 T2)). now destruct destArity.
+Qed.
+
+Lemma closedn_All_local_closed:
+  forall (cf : checker_flags) (Σ : global_context) (Γ : context) (ctx : list context_decl)
+         (wfΓ' : wf_local Σ (Γ ,,, ctx)),
+    All_local_env_over typing
+    (fun (Σ0 : global_context) (Γ0 : context) (_ : wf_local Σ0 Γ0) (t T : term) (_ : Σ0;;; Γ0 |- t : T) =>
+       closedn #|Γ0| t && closedn #|Γ0| T) Σ (Γ ,,, ctx) wfΓ' ->
+    closedn_ctx 0 Γ && closedn_ctx #|Γ| ctx.
+Proof.
+  intros cf Σ Γ ctx wfΓ' al.
+  induction Γ. simpl.
+  induction ctx using rev_ind. constructor.
+  depelim al. destruct ctx; discriminate.
+  unfold app_context in x1.
+Admitted.
+
+Lemma closedn_ctx_cons n d Γ : closedn_ctx n (d :: Γ) -> closedn_ctx n Γ && closed_decl (n + #|Γ|) d.
+Proof.
+  unfold closedn_ctx.
+  simpl. rewrite mapi_app. rewrite forallb_app.
+  move/andP => [] -> /=. now rewrite Nat.add_0_r List.rev_length andb_true_r.
+Qed.
+
+Lemma closedn_mkProd_or_LetIn (Γ : context) d T :
+    closed_decl #|Γ| d ->
+    closedn (S #|Γ|) T -> closedn #|Γ| (mkProd_or_LetIn d T).
+Proof.
+  destruct d as [na [b|] ty]; simpl in *. unfold closed_decl.
+  simpl. now move/andP => [] -> ->.
+  simpl. now move/andP => [] /= _ -> ->.
+Qed.
+
+Lemma closedn_mkLambda_or_LetIn (Γ : context) d T :
+    closed_decl #|Γ| d ->
+    closedn (S #|Γ|) T -> closedn #|Γ| (mkLambda_or_LetIn d T).
+Proof.
+  destruct d as [na [b|] ty]; simpl in *. unfold closed_decl.
+  simpl. now move/andP => [] -> ->.
+  simpl. now move/andP => [] /= _ -> ->.
+Qed.
+
+Lemma closedn_it_mkProd_or_LetIn
+      (Γ : context) (ctx : list context_decl) T :
+    closedn_ctx #|Γ| ctx ->
+    closedn (#|Γ| + #|ctx|) T -> closedn #|Γ| (it_mkProd_or_LetIn ctx T).
+Proof.
+  induction ctx in Γ, T |- *. simpl.
+  - now rewrite Nat.add_0_r.
+  - move/closedn_ctx_cons/andP => [] cctx ca cT.
+    apply (IHctx Γ (mkProd_or_LetIn a T) cctx).
+    simpl in cT. rewrite <- app_length.
+    eapply closedn_mkProd_or_LetIn;
+      now rewrite app_length // plus_n_Sm.
+Qed.
+
+Lemma closedn_it_mkLambda_or_LetIn
+      (Γ : context) (ctx : list context_decl) T :
+    closedn_ctx #|Γ| ctx ->
+    closedn (#|Γ| + #|ctx|) T -> closedn #|Γ| (it_mkLambda_or_LetIn ctx T).
+Proof.
+  induction ctx in Γ, T |- *. simpl.
+  - now rewrite Nat.add_0_r.
+  - move/closedn_ctx_cons/andP => [] cctx ca cT.
+    apply (IHctx Γ (mkLambda_or_LetIn a T) cctx).
+    simpl in cT. rewrite <- app_length.
+    eapply closedn_mkLambda_or_LetIn;
+      now rewrite app_length // plus_n_Sm.
+Qed.
 
 Lemma typecheck_closed `{cf : checker_flags} :
   env_prop (fun Σ Γ t T =>
@@ -155,29 +236,29 @@ Proof.
   { repeat red. intros. destruct t; red in X0; eauto. }
 
   apply typing_ind_env; intros * wfΣ Γ wfΓ *; simpl; intros; rewrite -> ?andb_and in *; try solve [intuition auto].
+
   - pose proof (nth_error_Some_length H).
-    elim (Nat.ltb_spec n #|Γ|); intuition.
-    eapply (All_local_env_lookup H0) in H. red in H.
-    destruct decl_body.
-    -- move/andb_and: H => [].
-       rewrite skipn_length; try lia; move=> Ht.
+    elim (Nat.ltb_spec n #|Γ|); intuition. clear H0.
+    eapply (nth_error_All_local_env_over H) in X0 as [HΓ Hdecl].
+    destruct lookup_wf_local_decl; cbn in *.
+    destruct decl as [na [b|] ty]; cbn in *.
+    -- move/andb_and: Hdecl => [] _.
+       rewrite skipn_length; try lia.
        move/(closedn_lift (S n)).
        now have->: #|Γ| - S n + S n = #|Γ| by lia.
-    -- move: H => [s].
-       move/andb_and => [Hty _].
-       move: Hty; rewrite skipn_length; try lia.
-       move/(closedn_lift (S n)).
-       have->: #|Γ| - S n + S n = #|Γ| by lia.
-       eauto.
+    -- rewrite andb_true_r in Hdecl.
+       move/(closedn_lift (S n)): Hdecl.
+       rewrite skipn_length; try lia.
+       now have->: #|Γ| - S n + S n = #|Γ| by lia.
 
   - intuition.
     generalize (closedn_subst [u] #|Γ| 0 B). rewrite Nat.add_0_r.
-    move=> Hs. apply: Hs => /=. rewrite H0 => //.
+    move=> Hs. apply: Hs => /=. rewrite H => //.
     rewrite Nat.add_1_r. auto.
 
   - rewrite closedn_subst_instance_constr.
-    eapply lookup_on_global_env in H0; eauto.
-    destruct H0 as [Σ' [HΣ' IH]].
+    eapply lookup_on_global_env in H; eauto.
+    destruct H as [Σ' [HΣ' IH]].
     repeat red in IH. destruct decl, cst_body. simpl in *.
     rewrite -> andb_and in IH. intuition.
     eauto using closed_upwards with arith.
@@ -211,14 +292,14 @@ Proof.
   - intuition auto. solve_all. unfold test_snd. simpl in *.
     toProp; eauto.
     apply closedn_mkApps; auto.
-    rewrite forallb_app. simpl. rewrite H5.
+    rewrite forallb_app. simpl. rewrite H4.
     rewrite forallb_skipn; auto.
-    now apply closedn_mkApps_inv in H10.
+    now apply closedn_mkApps_inv in H9.
 
-  - intuition.
+  - intuition auto.
     apply closedn_subst0.
-    simpl. apply closedn_mkApps_inv in H3.
-    rewrite forallb_rev H2. apply H3.
+    simpl. apply closedn_mkApps_inv in H2.
+    rewrite forallb_rev H1. apply H2.
     rewrite closedn_subst_instance_constr.
     destruct isdecl as [isdecl Hpdecl].
     eapply declared_inductive_inv in isdecl; eauto.
@@ -227,8 +308,8 @@ Proof.
     red in isdecl.
     destruct decompose_prod_assum eqn:Heq.
     destruct isdecl as [[s Hs] Hc]. simpl in *.
-    rewrite <- Hc in H1. rewrite <- H1 in Hs.
-    rewrite andb_true_r in Hs. rewrite List.rev_length.
+    rewrite <- Hc in H0. rewrite List.rev_length H0.
+    rewrite andb_true_r in Hs.
     eauto using closed_upwards with arith.
 
   - split. solve_all.
@@ -256,21 +337,26 @@ Proof.
     subst types. rewrite app_context_length in H0.
     rewrite Nat.add_comm in H0.
     now eapply closedn_lift_inv in H0.
-  - destruct X1; intuition eauto.
-    destruct B; simpl in i; destruct i. constructor.
-    destruct s. rewrite andb_true_r in p. intuition auto.
+
+  - destruct X2; intuition eauto.
+    + destruct i as [[u [ctx [Heq Hi]]] Hwfi]. simpl in Hwfi.
+      generalize (destArity_spec [] B). rewrite Heq.
+      simpl; intros ->.
+      apply closedn_All_local_closed in Hwfi. move/andP: Hwfi => [] clΓ clctx.
+      apply closedn_it_mkProd_or_LetIn => //.
+    + destruct s. rewrite andb_true_r in p. intuition auto.
 Qed.
 
 Lemma declared_decl_closed `{checker_flags} Σ cst decl :
   wf Σ ->
   lookup_env (fst Σ) cst = Some decl ->
-  on_global_decl (fun Σ Γ b t => option_default (closedn #|Γ|) b true && closedn #|Γ| t) Σ decl.
+  on_global_decl (fun Σ Γ b t => closedn #|Γ| b && option_default (closedn #|Γ|) t true) Σ decl.
 Proof.
   intros.
   eapply weaken_lookup_on_global_env; try red; eauto.
   eapply on_global_decls_impl; cycle 1.
   apply (env_prop_sigma _ typecheck_closed _ X).
-  red; intros. unfold lift_typing in *. destruct t; intuition auto with wf.
+  red; intros. unfold lift_typing in *. destruct T; intuition auto with wf.
   destruct X1 as [s0 Hs0]. simpl. toProp; intuition.
 Qed.
 
