pcuic/theories/PCUICValidity.v
@@ -1,85 +1,42 @@
+From Equations Require Import Equations.
 From Coq Require Import Bool String List Program BinPos Compare_dec Omega.
 From Template Require Import utils.
 From PCUIC Require Import PCUICAst PCUICAstUtils PCUICInduction PCUICLiftSubst PCUICTyping. (* PCUICWeakening. *)
 Require Import ssreflect.
 Existing Instance config.default_checker_flags.
-Lemma type_local_env_isdecl Σ n Γ :
-  forall isdecl : n < #|Γ|, All_local_env (lift_typing typing) Σ Γ ->
-  { Γ' : _ & { Γ'' : _ &
-                    { _ : type_local_decl Σ Γ'' (safe_nth Γ (exist _ n isdecl)) &
-                    Γ = Γ' ++ Γ'' /\ #|Γ'| = S n } } }.
-Proof. Admitted.
 
-Definition property :=
-  forall (Σ : global_context) (Γ : context),
-    All_local_env (lift_typing typing) Σ Γ -> forall t T : term, typing Σ Γ t T -> Type.
+Definition isWfArity_or_Type Σ Γ T : Type := (isWfArity typing Σ Γ T + isType Σ Γ T).
 
-(* Definition lookup_wf_local Σ Γ (wfΓ : wf_local Σ Γ) (n : nat | n < #|Γ|) : *)
-(*   { wf : wf_local Σ (skipn (S n) Γ) & *)
+(* Definition isWfArity Σ (Γ : context) T := *)
+(*   forall ctx s, destArity [] T = Some (ctx, s) -> All_local_env (lift_typing typing) Σ (Γ ,,, ctx). *)
 
-(*          let decl := safe_nth Γ n in *)
-(*          typing Σ (skipn (S n) Γ) *)
-(*          Q \Sigma \Gamma *)
+Lemma isWfArity_or_Type_lift Σ n Γ ty : isWfArity_or_Type Σ (skipn n Γ) ty -> isWfArity_or_Type Σ Γ (lift0 n ty).
+Proof.
+  intros [|]. red in i. left. intros ctx s Heq.
+  (* Needs weakening lemmas *) admit.
+  destruct i as [u Hu].
+  right. exists u. admit. (* Weakening *)
+Admitted.
 
-
-
-(* Definition on_wf_local_decl Σ Γ (wfΓ : wf_local Σ Γ) (P : property) d := *)
-(*   match d.(decl_body) with *)
-(*   | Some b => Q Σ Γ b (Some d.(decl_type)) *)
-(*   | None => P Σ Γ d.(decl_type) None *)
-(*   end. *)
-
-(* Lemma nth_error_All_local_env_over {P Q Σ Γ n} (isdecl : n < #|Γ|) (wfΓ : All_local_env P Σ Γ) : *)
-(*   All_local_env_over P Q Σ Γ wfΓ -> *)
-(*   on_some (on_local_decl (fun Σ Γ t T => P Σ (skipn (S n) Γ)) (nth_error Γ n)). *)
-(* Proof. *)
-(*   induction 1 in n, isdecl |- *. red; simpl. *)
-(*   - destruct n; simpl; inv isdecl. *)
-(*   - destruct n. red; simpl. red. simpl. apply t0. *)
-(*     simpl. apply IHX. simpl in isdecl. lia. *)
-(*   - destruct n. auto. *)
-(*     apply IHX. simpl in *. lia. *)
-(* Qed. *)
-
-(* Require Import LibHypsNaming. *)
-From Equations Require Import Equations.
+ (* Require Import LibHypsNaming. *)
 Theorem validity :
-  env_prop (fun Σ Γ t T => isType_or_Sort Σ Γ T).
+  env_prop (fun Σ Γ t T => isWfArity_or_Type Σ Γ T).
 Proof.
   apply typing_ind_env; intros; rename_all_hyps.
 
-  - induction X. destruct n; discriminate.
-    simpl in *. destruct tu as [u Hu]. simpl in *.
-    destruct n. simpl in *. noconf heq_nth_error.
-    simpl. red. right. exists u. admit.
-
-
-    destruct decl as [na' [b|] ty].
+  - destruct (nth_error_All_local_env_over heq_nth_error X) as [HΓ' Hd].
     destruct decl as [na [b|] ty]; cbn -[skipn] in *.
-    + destruct Hd as [Hty|[u Hu]].
-      ++ left; destruct ty; simpl in *; now destruct Hty.
-      ++ right. exists u.
-         (* epose proof (weakening _ _ (firstn (S n) Γ) _ _ _ _ Hu) as Hw. *)
-         (* rewrite [_ ,,, _]firstn_skipn in Hw. *)
-         (* rewrite firstn_length_le in Hw. apply nth_error_Some_length in heq_nth_error. auto with arith. *)
-         (* apply Hw. *) admit.
-    + simpl in *. destruct Hd as [u [Hs|Hty]].
+    now apply isWfArity_or_Type_lift.
+    destruct lookup_wf_local_decl; cbn -[skipn] in *.
+    destruct o. right. exists x0. admit. (* Weakening *)
 
-    pose proof (All_local_env_lookup HΓ0 heq_nth_error) as Hd.
-    red in Hd |- *. destruct decl as [na [b|] ty]; cbn -[skipn] in *.
-    + destruct Hd as [Hty|[u Hu]].
-      ++ left; destruct ty; simpl in *; now destruct Hty.
-      ++ right. exists u.
-         (* epose proof (weakening _ _ (firstn (S n) Γ) _ _ _ _ Hu) as Hw. *)
-         (* rewrite [_ ,,, _]firstn_skipn in Hw. *)
-         (* rewrite firstn_length_le in Hw. apply nth_error_Some_length in heq_nth_error. auto with arith. *)
-         (* apply Hw. *) admit.
-    + simpl in *. destruct Hd as [u [Hs|Hty]].
+  - left. intros ctx s. simpl. intros [= <- <-]. apply HΓ.
+  - left. intros ctx s. intros [= <- <-]. apply HΓ.
+  - destruct X3. left. intros ctx s. simpl. intros.
+    apply All_local_env_app_inv; split; auto.
+    specialize (i ctx s). forward i.
 
 
-  - exists (succ_sort (succ_sort s)). constructor.
-  - now exists s.
-  - eexists. constructor.
   - econstructor. constructor; eauto.
     destruct H2 as [s Hs]. constructor. auto. 
     eexists. eauto.
